crates/synch-verified/src/origin.rs
@@ -67,6 +67,7 @@ mod tests {
         keys: Vec<Vec<u8>>,
     }
     impl Crypto for Point {
+        host_unexpected!(verify_ed25519);
         type Error = &'static str;
         fn validate_ed25519(&mut self, bytes: &[u8]) -> Result<bool, Self::Error> {
             self.keys.push(bytes.to_vec());
